\documentclass{article}
\usepackage{mathtools}
\usepackage{qtree}
\usepackage{hyperref}
 \usepackage{url}
\usepackage{amsmath}
\DeclarePairedDelimiter{\ceil}{\lceil}{\rceil}
\DeclarePairedDelimiter{\floor}{\lfloor}{\rfloor}
\usepackage [USenglish]{babel}
\usepackage{amssymb}
\usepackage{amsmath} 
\usepackage{graphicx}
\graphicspath{ {images/} }



\usepackage{color}

\definecolor{pblue}{rgb}{0.13,0.13,1}
\definecolor{pgreen}{rgb}{0,0.5,0}
\definecolor{pred}{rgb}{0.9,0,0}
\definecolor{pgrey}{rgb}{0.46,0.45,0.48}

\usepackage{listings}
\lstset{language=C,
	showspaces=false,
	showtabs=false,
	breaklines=true,
	showstringspaces=false,
	breakatwhitespace=true,
	commentstyle=\color{pgreen},
	keywordstyle=\color{pblue},
	stringstyle=\color{pred},
	basicstyle=\ttfamily,
	moredelim=[is][\textcolor{pgrey}]{\%\%}{\%\%}
}

 \title{Homework \#3}
 \date{\today}
 \author{Paolo Grignaffini (ID: 800673343)}
\begin{document}
	\maketitle
	
\section*{Exercise 1}
\paragraph{}~\\~\\
$(A \land B) \lor (B \land C)$\\
\\
The models that make this sentence true are: 6
\begin{itemize}
	\item $A,B,C,D$
	\item $A,B,C,\lnot D$
	\item $A,B,\lnot C,D$
	\item $A,B,\lnot C,\lnot D$
	\item$\lnot A,B,C,D$
	\item $\lnot A, B,C, \lnot D$
\end{itemize}


$(A \lor B)$\\
The models that make this sentence true are: 12
\begin{itemize}
\item $\lnot A, B, C, D$
\item $A, \lnot B, C, D$
\item $A, B, C, D$
\item $\lnot A, B, \lnot C, D$
\item $A, \lnot B, \lnot C, D$
\item $A, B, \lnot C, D$
\item $\lnot A, B, C, \lnot D$
\item $A, \lnot B, C, \lnot D$
\item $A, B, C, \lnot D$
\item $\lnot A, B, \lnot C, \lnot D$
\item $A, \lnot B, \lnot C, \lnot D$
\item $A, B, \lnot C, \lnot D$
\end{itemize}

$(A \iff B) \iff C$\\
The models that make this sentence true are: 8
\begin{itemize}
\item $A,B,C,D$
\item $\lnot A, \lnot B, \lnot C,D$
\item $A,B,C,\lnot D$
\item $\lnot A, \lnot B, \lnot C, \lnot D$
\item $A,\lnot B, \lnot C,D$
\item $\lnot A, B, \lnot C,D$
\item $A,\lnot B, \lnot C,\lnot D$
\item $\lnot A, B, \lnot C,\lnot D$
\end{itemize}

\section*{Exercise 2}
\paragraph{}~\\~\\
$Smoke \implies Smoke$\\
Possible Interpretations:\\
$True \implies True$, which is $True$\\
$False \implies False$, which is $True$\\
Therefore the formula is valid and satisfiable.\\
\\
$(Smoke \implies Fire) \implies (\lnot Smoke \implies \lnot Fire)$\\
Possible Interpretations:\\
$(True \implies True) \implies (False \implies False)$, which is $True$\\
$(True \implies False) \implies (False \implies True)$, which is $True$\\
$(False \implies True) \implies (True \implies False)$, which is $False$\\
$(False \implies False) \implies (True \implies True)$, which is $True$\\
We found an Interpretation that is not a Model of the formula, therefore the formula is satisfiable but not valid.\\
\\
$((Smoke \land Heat) \implies Fire) \iff ((Smoke \implies Fire) \lor (Heat \implies Fire))$\\
Possible Interpretations:\\
$((True \land True) \implies True) \iff ((True \implies True) \lor (True \implies True))$, which is $True$\\
$((True \land True) \implies False) \iff ((True \implies False) \lor (True \implies False))$, which is $True$\\
$((True \land False) \implies True) \iff ((True \implies True) \lor (False \implies True))$, which is $True$\\
$((True \land False) \implies False) \iff ((True \implies False) \lor (False \implies False))$, which is $True$\\
$((False \land True) \implies True) \iff ((False \implies True) \lor (True \implies True))$, which is $True$\\
$((False \land True) \implies False) \iff ((False \implies False) \lor (True \implies False))$, which is $True$\\
$((False \land False) \implies True) \iff ((False \implies True) \lor (False \implies True))$, which is $True$\\
$((False \land False) \implies False) \iff ((False \implies False) \lor (False \implies False))$, which is $True$\\
Therefore the formula is valid and satisfiable.\\

\section*{Exercise 3}
\paragraph{}~\\~\\
\begin{equation}
\begin{aligned}
&((A \land B) \lor (B \land C)) \implies (D \land E)\\
&\lnot ((A \land B) \lor (B \land C)) \lor (D \land E)\\
&(\lnot (A \land B) \land \lnot(B \land C)) \lor (D \land E)\\
&((\lnot A \lor \lnot B) \land (\lnot B \lor \lnot C)) \lor (D \land E)\\
&(D \land E) \lor ((\lnot A \lor \lnot B) \land (\lnot B \lor \lnot C))\\
&(D \lor ((\lnot A \lor \lnot B) \land (\lnot B \lor \lnot C))\land (E \lor ((\lnot A \lor \lnot B) \land (\lnot B \lor \lnot C))\\
&(\lnot A \lor \lnot B \lor D) \land (\lnot B \lor \lnot C \lor D)\land (\lnot A \lor \lnot B \lor E) \land (\lnot B \lor \lnot C \lor E)
\end{aligned}
\end{equation}
\newpage
\section*{Exercise 4}
\paragraph{}~\\~\\
\begin{equation}
\begin{aligned}
&\frac{A,B~~~~~~~~~~A\land B \implies L} {L} \text{\{\}}\\
& \\
&\frac{B,L~~~~~~~~~~L\land B \implies M} {M} \text{\{\}}\\
& \\
&\frac{L,M~~~~~~~~~~L\land M \implies P} {P} \text{\{\}}\\
& \\
&\frac{P~~~~~~~~~~P \implies Q} {Q} \text{\{\}}\\
& \\
&Q
\end{aligned}
\end{equation}

\section*{Exercise 5}
\paragraph{}~\\~\\
The problem can be represented by the following $KB$:\\
\\
$\forall x \exists y | \text{marriage}(x,y)$\\
 $\forall x(\forall y| \text{marriage}(x,y)\land \forall z| \text{marriage}(x,z)) \implies y = z$\\
$\text{marriage}(x,y) \implies (\text{preference}(x,y) \land \text{preference}(y,x))$\\
$\text{marriage}(x,y) \implies \text{marriage}(y,x)$\\
\\
Where the formula: marriage($x,y$) means that $x$ is married with $y$.\\
The formula: preference($x,y$) means that $x$ has expressed a preference in order to marry $y$.

\section*{Exercise 6}
\paragraph{}~\\~\\
$P(A,B,C), P(x,y,z)$\\
$P(A,B,C), P(A,B,C)$\\
\textbf{mgu} = $\{x/A, y/B, z/C\}$\\
\\
$Q(y, G(A,B)), Q(G(x,x), y)$\\
$Q(G(x,x), G(A,B)), Q(G(x,x), G(x,x)~~~~~~~~~\eta = \{y/G(x,x)\}$\\
$Q(G(A,A), G(A,B)), Q(G(A,A), G(A,A)~~~~~~\eta = \{x/A\}$\\
\textbf{mgu} doesn't exist.\\
\\
$O(F(y), x), O(F(x), J)$\\
$O(F(x), x), O(F(x), J)~~~~~~\eta = \{y/x\}$\\
$O(F(J), J), O(F(J), J)~~~~~~\eta = \{x/J\}$\\
\textbf{mgu} = $\{y/x, x/J\}$\\
\\
$K(F(y),y), K(x,x)$\\
$K(F(y),y), K(F(y),F(y))~~~~~~\eta = \{x/F(y)\}$\\
\textbf{mgu} doesn't exist.\\

\section*{Exercise 7}
\paragraph{}~\\~\\
Horse($x$) $\implies$ Animal($x$)\\
Cow($x$) $\implies$ Animal($x$)\\
Pig($x$) $\implies$ Animal($x$)\\
Horse($x$) $\land$ Offspring($x, y$) $\implies$ Horse($y$)\\
Horse(Bluebeard)\\
Parent(Charlie, Bluebeard)\\
Offspring($x, y$) $\iff$ Parent($y,x$)\\
Mammal($x$) $\implies$ $\exists y$ Parent($x,y$)\\
Mammal($x$) $\implies$ Animal($x$)\\
\\
``Charlie is an horse and is an offspring of Bluebeard":\\
\\
\begin{equation}
\begin{aligned}
& \frac{\text{Parent(Charlie, Blue)}, \text{Offspring}(x,y) \iff \text{Parent}(y,x)}{}\\
& \frac{\text{Parent(Charlie, Blue)}, \text{Offspring(Blue, Charlie)} \iff \text{Parent(Charlie, Blue)}}{ \text{Offspring(Blue, Charlie)}}\eta = \{y/\text{Charlie}, x/\text{Blue}\}\\
&\\
&\text{Offspring(Blue, Charlie)} \land \text{Horse(Blue), } \text{Horse}(x) \land \text{Offspring}(x,y) \implies \text{Horse}(y)\\
&\frac{\text{Offspring(Blue, Charlie)} \land \text{Horse(Blue), } \text{Horse(Blue)} \land \text{Offspring(Blue, Charlie)} \implies \text{Horse(Charlie)}}{\text{Horse(Charlie)}~~~~~~~~~~~\eta = \{y/\text{Charlie}, x/\text{Blue}\}}
\end{aligned}
\end{equation}
\\
``Is Charlie a cow?":\\
Since doesn't exist any relation that states that a horse is not a cow and a cow is not a horse we cannot make any assumptions, therefore with the KB that we have we cannot answer that question.

\section*{Exercise 8}
\paragraph{}~\\~\\
We can prove that a ground sentence is \textbf{\textit{valid} or \textbf{unsatisfiable}} in the following way:\\
\begin{itemize}
	\item Negate the desired conclusion, after converting it into CNF (in our case the ground sentence)
	\item Apply the resolution rule in order to derive new axioms
	\subitem If a contradiction is derived then the ground sentence is valid
	\subitem If we cannot apply the rules anymore and a contradiction has not
	\subitem been found, then the ground sentence is unsatisfiable
\end{itemize}
\end{document}